\documentclass[11pt,a4paper]{article}

\usepackage{../ve230}

\author{\href{liuyh615@sjtu.edu.cn}{Yihao Liu} (515370910207)}
\semester{Summer}
\year{2019}
\subtitle{Homework}
\subtitlenumber{5}
\blockinfo{}

\usetikzlibrary{positioning}

\begin{document}

\maketitle

\subsection{5-7}
\begin{enumerate}[label=\alph*)]
\item
$$\exp\left[-\frac{\sigma}{\varepsilon}t\right]=0.01,$$
$$t=-\frac{\varepsilon_0\varepsilon_r}{\sigma}\ln0.01\approx \SI{4.89e-12}{\second}.$$
\item
$$\Delta W=\exp\left[-\frac{\sigma}{\varepsilon}t\right]^2=\num{1e-4}.$$
The energy are transformed into heat energy.
\item
$$\frac{Q}{\varepsilon_0}=E\cdot 4\pi r^2,$$
$$E=\frac{Q}{4\pi r^2\varepsilon_0},$$
$$W=\int_0^{Q_0} VdQ=\int_0^{Q_0}\int_R^\infty-EdrdQ=\int_0^{Q_0}\frac{Q}{4\pi R\varepsilon_0}dQ=\frac{Q_0^2}{8\pi R\varepsilon_0}\approx\SI{4.494e4}{\joule}.$$
\end{enumerate}

\subsection{5-10}
\begin{enumerate}[label=\alph*)]
\item
$$\sigma(y)=\frac{\sigma_2-\sigma_1}{d}y+\sigma_1,$$
$$\frac{dy}{d\sigma}=\frac{d}{\sigma_2-\sigma_1},$$
$$R=\int_0^d\frac{1}{\sigma S}dy=\frac{1}{S}\int_{\sigma_1}^{\sigma_2}\frac{1}{\sigma}d\sigma\cdot\frac{dy}{d\sigma}=\frac{d}{S(\sigma_2-\sigma_1)}\int_{\sigma_1}^{\sigma_2}\frac{1}{\sigma}d\sigma=\frac{d}{S(\sigma_2-\sigma_1)}\ln\frac{\sigma_2}{\sigma_1}.$$
\item
$$J=\frac{V}{RS}=\frac{V(\sigma_2-\sigma_1)}{d\ln\frac{\sigma_2}{\sigma_1}},$$
$$\rho_b=-\varepsilon_0E(0)=-\varepsilon_0\frac{J}{\sigma_1}=-\frac{\varepsilon_0V(\sigma_2-\sigma_1)}{\sigma_1d\ln\frac{\sigma_2}{\sigma_1}},$$
$$\rho_t=\varepsilon_0E(d)=\varepsilon_0\frac{J}{\sigma_2}=\frac{\varepsilon_0V(\sigma_2-\sigma_1)}{\sigma_2d\ln\frac{\sigma_2}{\sigma_1}}.$$
\item
$$\rho=\frac{d}{dy}\varepsilon_0E=\frac{d}{dy}\left[-\varepsilon_0J\cdot\frac{d}{\sigma(y)}\right]=\frac{\varepsilon_0J(\sigma_2-\sigma_1)d}{[(\sigma_2-\sigma_1)y+d\sigma_1]^2}=\frac{\varepsilon_0V(\sigma_2-\sigma_1)^2}{[(\sigma_2-\sigma_1)y+d\sigma_1]^2\ln\frac{\sigma_2}{\sigma_1}}.$$
$$Q=(\rho_b+\rho_t)S=\frac{\varepsilon_0V(\sigma_2-\sigma_1)S}{d\ln\frac{\sigma_2}{\sigma_1}}\left(\frac{1}{\sigma_2}-\frac{1}{\sigma_1}\right).$$
\end{enumerate}

\subsection{5-16}
$$\frac{1}{R^2(1+k/R)}=\frac{1}{R(R+k)}=\frac{1}{k}\left(\frac{1}{R}-\frac{1}{R+k}\right),$$
$$R_0=\int_{R_1}^{R_2}\frac{1}{\sigma\cdot 4\pi R^2}dR=\frac{1}{4\pi\sigma_0k}\int_{R_1}^{R_2}\left(\frac{1}{R}-\frac{1}{R+k}\right)dR=\frac{1}{4\pi\sigma_0k}\ln\frac{R}{R+k}\bigg|_{R_1}^{R_2}=\frac{1}{4\pi\sigma_0k}\ln\frac{R_2(R_1+k)}{R_1(R_2+k)}.$$

\subsection{5-22}
\begin{enumerate}[label=\alph*)]
\item
$$V=\frac{V_0}{a}x.$$
\item
$$\mathbf{E}=-\nabla V=-\frac{V_0}{a}\mathbf{a}_x.$$
$$\mathbf{J}=\sigma \mathbf{E}=-\frac{\sigma V_0}{a}\mathbf{a}_x.$$
\end{enumerate}

\subsection{6-2}
\begin{enumerate}[label=\alph*)]
\item
$$\mathbf{F}=-e(\mathbf{E}+\mathbf{v}\times\mathbf{B})=-e(E_0-u_0B_0)\mathbf{a}_z.$$
If $E_0>u_0B_0$, the electron moves on -z and y direction;

If $E_0<u_0B_0$, the electron moves on z and y direction;

If $E_0=u_0B_0$, the electron moves on y direction.
\item
$$\mathbf{F}=-e(\mathbf{E}+\mathbf{v}\times\mathbf{B})=e(E_0\mathbf{a}_z+u_0B_0\mathbf{a}_x)\mathbf{a}_z.$$
If $E_0>u_0B_0$, the electron moves on x-z direction, closer to z direction and y direction;

If $E_0<u_0B_0$, the electron moves on x-z direction, closer to x direction and y direction;

If $E_0=u_0B_0$, the electron moves on the midline of x-z direction and y direction.
\end{enumerate}

\subsection{6-12}
$$\mathbf{B}=\mathbf{a}_x\cdot\frac{\mu_0Ib^2N}{2}\left\{[(x+d/2)^2+b^2]^{-3/2}+[(x-d/2)^2+b^2]^{-3/2}\right\}.$$
\begin{enumerate}[label=\alph*)]
\item
$$\mathbf{B}(x=0)=\mathbf{a}_x\cdot\mu_0Ib^2N[(d/2)^2+b^2]^{-3/2}.$$
\item
$$\frac{dB_x}{dx}=\frac{\mu_0Ib^2N}{2}\left\{-\frac{3}{2}[(x+d/2)^2+b^2]^{-5/2}(2x+d)-\frac{3}{2}[(x-d/2)^2+b^2]^{-5/2}(2x-d)\right\},$$
$$\frac{dB_x(0)}{dx}=\frac{\mu_0Ib^2N}{2}\left\{-\frac{3}{2}[(d/2)^2+b^2]^{-5/2}d-\frac{3}{2}[(d/2)^2+b^2]^{-5/2}(-d)\right\}=0.$$
\item
\begin{align*}
\frac{d^2B_x}{dx^2}=\frac{3\mu_0Ib^2N}{4}&\left\{\frac{5}{2}[(x+d/2)^2+b^2]^{-7/2}(2x+d)^2-2[(x+d/2)^2+b^2]^{-5/2}\right.\\
&\left.+\frac{5}{2}[(x-d/2)^2+b^2]^{-7/2}(2x-d)^2-2[(x-d/2)^2+b^2]^{-5/2}\right\},
\end{align*}
$$\frac{d^2B_x(0)}{dx^2}=\frac{3\mu_0Ib^2N}{4}\left\{5d^2[(d/2)^2+b^2]^{-7/2}-4[(d/2)^2+b^2]^{-5/2}\right\}=0,$$
$$5d^2[(d/2)^2+b^2]^{-1}-4=0,$$
$$b=d.$$
\end{enumerate}

\subsection{6-24}
\begin{enumerate}[label=\alph*)]
\item
\begin{align*}
V_m&=\int\frac{I\mathbf{a}_n\cdot\mathbf{a}_R}{4\pi(z^2+r^2)} dS\\
&=\int_0^{2\pi}\int_0^b \frac{I}{4\pi(z^2+r^2)}\frac{z}{\sqrt{z^2+r^2}}rdrd\theta\\
&=\frac{I}{8\pi}\int_0^{2\pi}\int_{z^2}^{z^2+b^2}z(z^2+r^2)^{-3/2}d(z^2+r^2)d\theta\\
&=\frac{I}{8\pi}\int_0^{2\pi}2[1-z(z^2+b^2)^{-1/2}]d\theta\\
&=\frac{I}{2}\left(1-\frac{z}{\sqrt{z^2+b^2}}\right).
\end{align*}
\item
\begin{align*}
\mathbf{B}&=-\mu_0\nabla V_m\\
&=-\mu_0\cdot\mathbf{a}_z\frac{I}{2}\left(-\frac{\sqrt{z^2+b^2}-2z\cdot\frac{1}{2}/\sqrt{z^2+b^2}\cdot z}{z^2+b^2}\right)\\
&=\mathbf{a}_z\frac{\mu_0I}{2}\left(\frac{z^2+b^2-z^2}{(z^2+b^2)^{3/2}}\right)\\
&=\mathbf{a}_z\frac{\mu_0Ib^2}{2(z^2+b^2)^{3/2}}.
\end{align*}
\end{enumerate}

\end{document}


