\documentclass[6pt,a4paper]{article}
\usepackage{../ve230}
\usetikzlibrary{positioning}

\begin{document}

\subsection{7-2}
\begin{align*}
\Phi&=\int\mathbf{B}d\mathbf{S}=\int_0^{0.2}\int_0^{0.6}3\cos\left(5\pi10^7t-\frac{2}{3}\pi x\right)dxdy\cdot10^{-6}\\&=\frac{\num{9e-7}}{\pi}[\sin(5\pi10^7t)+\sin(0.4\pi-5\pi10^7t)]\si{\weber}.
\end{align*}
$$V=-\frac{d\Phi}{dt}=-45[\cos(5\pi10^7t)-\cos(0.4\pi-5\pi10^7t)],$$
$$i=\frac{V}{2R}=-1.5[\cos(5\pi10^7t)-\cos(0.4\pi-5\pi10^7t)].$$

\subsection{7-6}
\begin{enumerate}[label=\alph*)]
\item
$$dR=\frac{2\pi r}{\sigma hdr},$$
$$V=\frac{d\Phi}{dt}=\frac{d(B_0\sin\omega t\cdot \pi r^2)}{dt}=B_0\omega\pi r^2\cos\omega t,$$
$$dP=\frac{V^2}{dR}=\frac{B_0^2\omega^2\pi^2 r^4\cos^2\omega t\cdot\sigma hdr}{2\pi r}=\frac{1}{2}B_0^2\omega^2\pi r^3h\sigma\cos^2\omega t\cdot dr,$$
$$P=\int dP=\int_0^R\frac{1}{2}B_0^2\omega^2\pi r^3h\sigma\cos^2\omega t\cdot dr=\frac{1}{8}B_0^2\omega^2\pi R^4h\sigma\cos^2\omega t,$$
$$\overline{P}=\frac{1}{2\pi}\int_0^{2\pi}\frac{1}{8}B_0^2\omega^2\pi R^4h\sigma\cos^2\omega t dt=\frac{1}{16}B_0^2\omega^2\pi R^4h\sigma.$$
\item
$$0.95\pi R^2=N\cdot \pi R'^2,$$
$$R'^2=\sqrt{\frac{0.95}{N}}R,$$
$$\overline{P'}=N\cdot\frac{1}{16}B_0^2\omega^2\pi R'^4h\sigma=\frac{0.95^2}{16N}B_0^2\omega^2\pi R^4h\sigma.$$
\end{enumerate}

\subsection{7-11}
$$\nabla\times\mathbf{E}=-\frac{\partial B}{\partial t},$$
$$\nabla\cdot(\nabla\times\mathbf{E})=-\frac{\partial}{\partial t}(\nabla\cdot\mathbf{B})=0.$$
So $\nabla\cdot\mathbf{B}$ is a constant, and $\mathbf{B}=\mathbf{0}$ in infinite distance, which means $\nabla\cdot\mathbf{B}=0$ at that point, so that $\nabla\cdot\mathbf{B}=0$ always stands.

$$\nabla\times\mathbf{H}=\mathbf{J}+\frac{\partial D}{\partial t},$$
$$\nabla\cdot(\nabla\times\mathbf{H})=\nabla\cdot\mathbf{J}+\frac{\partial}{\partial t}(\nabla\cdot\mathbf{D})=-\frac{\partial\rho}{\partial t}+\frac{\partial}{\partial t}(\nabla\cdot\mathbf{D}),$$
$$\nabla\cdot\mathbf{D}=\rho.$$

\subsection{7-12}
$$\left\{\begin{aligned}
\nabla^2V-\mu\varepsilon\frac{\partial^2V}{\partial t^2}=-\frac{\rho}{\varepsilon} \\
\nabla^2\mathbf{A}-\mu\varepsilon\frac{\partial^2\mathbf{A}}{\partial t^2}=-\mu\mathbf{J}
\end{aligned}\right.\Longrightarrow\left\{\begin{aligned}
\rho=\varepsilon\left(\mu\varepsilon\frac{\partial^2V}{\partial t^2}-\nabla^2V\right) \\
\mathbf{J}=\frac{1}{\mu}\left(\mu\varepsilon\frac{\partial^2\mathbf{A}}{\partial t^2}-\nabla^2\mathbf{A}\right) \\
\end{aligned}\right.,$$
$$-\frac{\partial\rho}{\partial t}=-\varepsilon\left(\mu\varepsilon\frac{\partial^3V}{\partial t^3}-\nabla^2\frac{\partial V}{\partial t}\right),$$
$$\nabla\cdot\mathbf{A}=-\mu\varepsilon\frac{\partial V}{\partial t},$$
$$\nabla\cdot\mathbf{J}=\frac{1}{\mu}\left(\mu\varepsilon\frac{\partial^2(\nabla\cdot\mathbf{A})}{\partial t^2}-\nabla^2(\nabla\cdot\mathbf{A})\right)=\varepsilon\left(\mu\varepsilon\frac{\partial^3V}{\partial t^3}-\nabla^2\frac{\partial V}{\partial t}\right),$$
$$\nabla\cdot \mathbf{J}=-\frac{\partial\rho}{\partial t}.$$

\subsection{7-14}
\begin{align*}
\mathbf{J}&=\nabla\times\mathbf{H}-\frac{\partial\mathbf{D}}{\partial t}\\
&=\frac{1}{\mu}\nabla\times\mathbf{B}-\varepsilon\frac{\partial\mathbf{E}}{\partial t}\\
&=\frac{1}{\mu}\nabla\times(\nabla\times\mathbf{A})+\varepsilon\nabla\frac{\partial V}{\partial t}+\varepsilon\frac{\partial^2\mathbf{A}}{\partial t^2}\\
&=\frac{1}{\mu}\nabla\times(\nabla\times\mathbf{A})-\frac{1}{\mu}\nabla(\nabla\cdot\mathbf{A})+\varepsilon\frac{\partial^2\mathbf{A}}{\partial t^2},
\end{align*}
$$\nabla^2\mathbf{A}-\mu\varepsilon\frac{\partial^2\mathbf{A}}{\partial t^2}=-\mu\mathbf{J}.$$
$$\rho=\nabla\cdot\mathbf{D}=\varepsilon\nabla\cdot\mathbf{E}=-\varepsilon\nabla^2 V-\varepsilon\frac{\partial}{\partial t}(\nabla\cdot\mathbf{A})=-\varepsilon\nabla^2 V+\varepsilon\frac{\partial}{\partial t}\mu\varepsilon\frac{\partial V}{\partial t},$$
$$\nabla^2V-\mu\varepsilon\frac{\partial^2V}{\partial t^2}=-\frac{\rho}{\varepsilon}.$$

\subsection{7-17}
\begin{enumerate}[label=\alph*)]
\item
$$E_{1t}=E_{2t},\quad B_{1n}=B_{2n}.$$
\item
$$D_{1n}=D_{2n},\quad H_{1t}=H_{2t}.$$
\end{enumerate}

\subsection{7-20}
Let $u=t\pm R\sqrt{\mu\epsilon}$, $f(u)=U(R,t)$,
$$\left(\frac{\partial u}{\partial R}\right)^2=\mu\varepsilon,\quad \left(\frac{\partial u}{\partial t}\right)^2=1.$$
$$\frac{\partial^2 U}{\partial R^2}-\mu\epsilon\frac{\partial^2 U}{\partial t^2}=\frac{\partial^2 f}{\partial u^2}\left(\frac{\partial u}{\partial R}\right)^2-\mu\epsilon\frac{\partial^2 f}{\partial u^2}\left(\frac{\partial u}{\partial t}\right)^2=0.$$

\subsection{7-24}
$$\nabla\times\mathbf{E}=-\frac{\partial\mathbf{B}}{\partial t}=-\mu\frac{\partial\mathbf{H}}{\partial t},$$
$$\nabla\times(\nabla\times\mathbf{E})=-\mu\frac{\partial}{\partial t}\left(\mathbf{J}+\frac{\partial\mathbf{D}}{\partial t}\right)=-\mu\frac{\partial\mathbf{J}}{\partial t}-\mu\varepsilon\frac{\partial^2\mathbf{E}}{\partial t^2},$$
$$\nabla\times(\nabla\times\mathbf{E})=\nabla(\nabla\cdot\mathbf{E})-\nabla^2\mathbf{E}=\frac{1}{\varepsilon}\nabla\rho-\nabla^2\mathbf{E},$$
$$\nabla^2\mathbf{E}=\frac{1}{\varepsilon}\nabla\rho+\mu\frac{\partial\mathbf{J}}{\partial t}+\mu\varepsilon\frac{\partial^2\mathbf{E}}{\partial t^2},$$
$$\nabla^2\mathbf{E}=\frac{1}{\varepsilon}\nabla\rho+\mu j\omega\mathbf{J}+\mu\varepsilon\omega^2\mathbf{E}.$$

$$\nabla\times\mathbf{H}=\mathbf{J}+\frac{\partial\mathbf{D}}{\partial t},$$
$$\nabla\times(\nabla\times\mathbf{H})=\nabla\times\mathbf{J}+\varepsilon\frac{\partial}{\partial t}(\nabla\times\mathbf{E})=\nabla\times\mathbf{J}-\mu\varepsilon\frac{\partial^2\mathbf{H}}{\partial t^2},$$
$$\nabla\times(\nabla\times\mathbf{H})=\nabla(\nabla\cdot\mathbf{H})-\nabla^2\mathbf{H}=-\nabla^2\mathbf{H},$$
$$\nabla^2\mathbf{H}=-\nabla\times\mathbf{J}+\mu\varepsilon\frac{\partial^2\mathbf{H}}{\partial t^2},$$
$$\nabla^2\mathbf{H}=-\nabla\times\mathbf{J}+\mu\varepsilon\omega^2\mathbf{H}.$$

\subsection{7-27}
\begin{align*}
\nabla\times\mathbf{E}&=\frac{1}{R^2\sin\theta}\begin{vmatrix}
\mathbf{a}_R & \mathbf{a}_\theta R & \mathbf{a}_\phi R\sin\theta \\
\frac{\partial}{\partial R} & \frac{\partial}{\partial\theta} & \frac{\partial}{\partial\phi} \\
0 & E_0\sin\theta e^{-jkR} & 0 \end{vmatrix}\\
&=\frac{1}{R^2\sin\theta}\left(\mathbf{a}_R\frac{\partial}{\partial\phi}E_0\sin\theta e^{-jkR}-\mathbf{a}_\phi R\sin\theta\frac{\partial}{\partial R}E_0\sin\theta e^{-jkR}\right)\\
&=\mathbf{a}_\phi\frac{-E_0jk\sin\theta e^{-jkR}}{R},
\end{align*}
$$\nabla\times\mathbf{E} = -\mu\frac{\partial\mathbf{H}}{\partial t}=-j\mu\omega\mathbf{H},$$
$$\mathbf{H}=\mathbf{a}_\phi\frac{E_0k\sin\theta e^{-jkR}}{\mu\omega R},\quad k=\omega\sqrt{\mu\varepsilon}.$$
$$\mathbf{H}(R)=\mathbf{a}_\phi\frac{E_0\sqrt{\mu\varepsilon}\sin\theta e^{-j\omega\sqrt{\mu\varepsilon}R}}{\mu R},$$
$$\mathbf{H}(R,t)=\text{Re}[\mathbf{H}(R)e^{j\omega t}]=\mathbf{a}_\phi\frac{E_0\sqrt{\mu\varepsilon}}{\mu R}\sin\theta\cos(\omega t-\omega\sqrt{\mu\varepsilon}R).$$

\subsection{7-29}

\begin{enumerate}[label=\alph*)]
\item
$$\nabla\times\mathbf{E}=-j\omega\mu_0\mathbf{H}=\omega^2\mu_0\varepsilon_0\nabla\times \pi_e,$$
$$\nabla\times(\mathbf{E}-\omega^2\mu_0\varepsilon_0\pi_e)=\mathbf{0},$$
$$\mathbf{E}=\omega^2\mu_0\varepsilon_0\pi_e+\mathbf{C}.$$
$$\nabla\times\mathbf{H}=j\omega\mathbf{D}=\omega^2\mu_0\varepsilon_0\nabla\times \pi_e,$$
$$\nabla\times(j\omega\varepsilon_0\nabla\times\pi_e)=j\omega\varepsilon_0(\omega^2\mu_0\varepsilon_0\pi_e+\frac{\mathbf{P}}{\varepsilon_0}+\mathbf{C}),$$
$$\nabla\times(\nabla\times\pi_e)=\nabla(\nabla\cdot\pi_e)-\nabla^2\pi_e=\omega^2\mu_0\varepsilon_0\pi_e+\frac{\mathbf{P}}{\varepsilon_0}+\mathbf{C},$$
$$\nabla^2\pi_e+\omega^2\mu_0\varepsilon_0\pi_e=\nabla(\nabla\cdot\pi_e)-\frac{\mathbf{P}}{\varepsilon_0}-\mathbf{C},$$
$$\mathbf{C}=\nabla(\nabla\cdot\pi_e),$$
$$\mathbf{E}=\omega^2\mu_0\varepsilon_0\pi_e+\nabla(\nabla\cdot\pi_e).$$
\item
$$k_0^2=\omega^2\mu_0\varepsilon_0,$$
$$\nabla^2\pi_e+k_0^2\pi_e=-\frac{\mathbf{P}}{\varepsilon_0}.$$
\end{enumerate}

\subsection{8-7}
Let $\phi=\omega_t-kz$,
$$\mathbf{E}(\phi)=\mathbf{a}_xE_{10}\sin\phi+\mathbf{a_y}E_{20}\sin(\phi+\psi),$$
$$\frac{E_x}{E_{10}}=\sin\phi,$$
$$\frac{E_y}{E_{20}}=\sin(\phi+\psi)=\sin\phi\cos\psi+\cos\phi\sin\psi=\frac{E_x}{E_{10}}\cos\psi+\sqrt{1-\left(\frac{E_x}{E_{10}}\right)^2}\sin\psi,$$
$$\left[\sqrt{1-\left(\frac{E_x}{E_{10}}\right)^2}\sin\psi\right]^2=\left(\frac{E_y}{E_{20}}\right)^2+\left(\frac{E_x}{E_{10}}\cos\psi\right)^2-2\left(\frac{E_y}{E_{20}}\right)\left(\frac{E_x}{E_{10}}\cos\psi\right),$$
$$\left(\frac{E_x}{E_{10}}\right)^2+\left(\frac{E_y}{E_{20}}\right)^2-2\frac{E_x}{E_{10}}\frac{E_y}{E_{20}}\cos\psi=\sin^2\psi,$$
$$\left(\frac{E_x}{E_{10}\sin\psi}\right)^2+\left(\frac{E_y}{E_{20}\sin\psi}\right)^2-2\frac{E_x}{E_{10}}\frac{E_y}{E_{20}}\frac{\cos\psi}{sin^2\psi}=1.$$

\subsection{8-9}
$$\nabla^2\mathbf{E}+k_c^2\mathbf{E}=0,$$
$$k_c=\omega\sqrt{\mu\varepsilon}=\beta-j\alpha,$$
$$\omega^2\mu\varepsilon=\omega^2\mu(\varepsilon-j\sigma/\omega)=\beta^2-\alpha^2-2j\alpha\beta,$$
$$\left\{\begin{aligned}
\beta^2+\alpha^2&=\omega^2\mu\sqrt{\varepsilon^2+\sigma^2/\omega^2}\\
\beta^2-\alpha^2&=\omega^2\mu\varepsilon\\
\end{aligned}\right.\Longrightarrow\left\{\begin{aligned}
\alpha&=\omega\sqrt{\frac{\mu\varepsilon}{2}}\left[\sqrt{1+\left(\frac{\sigma^2}{\omega\varepsilon}\right)^2}-1\right]^{1/2}\\
\beta&=\omega\sqrt{\frac{\mu\varepsilon}{2}}\left[\sqrt{1+\left(\frac{\sigma^2}{\omega\varepsilon}\right)^2}+1\right]^{1/2}
\end{aligned}\right..$$

\subsection{8-14}
$$f_{max}=\frac{1}{2\pi}\sqrt{\frac{N_{max}e^2}{m\varepsilon_0}},$$
$$\varepsilon_{min}=\varepsilon_0\left[1-\left(\frac{f_{max}}{f}\right)^2\right],$$
$$\frac{1}{\sin\theta_i}=\sqrt{\frac{\varepsilon_0}{\varepsilon_{min}}},$$
$$\varepsilon_{min}=\varepsilon_0\sin^2\theta_i=\varepsilon_0\left[1-\left(\frac{f_{max}}{f}\right)^2\right],$$
$$f=\frac{f_{max}}{\cos\theta_i}=\frac{1}{2\pi\cos\theta_i}\sqrt{\frac{N_{max}e^2}{m\varepsilon_0}}.$$

\subsection{8-15}
\begin{enumerate}[label=\alph*)]
\item
$$u_g=\frac{dw}{d\beta}=\frac{d}{d\beta}(\beta u_p)=u_p+\beta\frac{du_p}{d\beta}.$$
\item
$$\lambda=\frac{2\pi}{\beta},$$
$$\frac{d\lambda}{d\beta}=\frac{d}{d\beta}\left(\frac{2\pi}{\beta}\right)=-\frac{2\pi}{\beta^2}=-\frac{\lambda}{\beta},$$
$$u_g=u_p+\beta\frac{du_p}{d\beta}=u_p+\beta\frac{du_p}{d\lambda}\cdot\frac{d\lambda}{d\beta}=u_p-\lambda\frac{du_p}{d\lambda}.$$
\end{enumerate}

\subsection{8-22}

\begin{enumerate}[label=\alph*)]
\item
$$\mathbf{E}_i(x,z)=\mathbf{a}_y10e^{-j(6x+8z)}=\mathbf{a}_yE_0e^{-jk_xx-jk_zz},$$
$$E_0=10\quad k_x=6,\quad k_z=8,$$
$$k=\sqrt{k_x^2+k_z^2}=10,$$
$$\lambda=\frac{2\pi}{k}=0.2\pi~\si{\m}\approx\SI{0.628}{\m},$$
$$f=\frac{c}{\lambda}=\SI{4.777e8}{\Hz}.$$
\item
$$\omega=2\pi f=\SI{3e9}{\radian\per\s},$$
$$\eta_0=\frac{\omega\mu}{k}=120\pi~\Omega,$$
$$\mathbf{E}_i(x,z,t)=\text{Re}[\mathbf{E}_i(x,z)e^{j\omega t}]=\mathbf{a_y}10\cos(\num{3e9}t-6x-8z)~\si{\V\per\m}.$$
$$\mathbf{a}_{n_i}=\mathbf{a}_x\cdot\frac{k_x}{k}+\mathbf{a}_z\cdot\frac{k_z}{k},$$
$$\mathbf{H}_i(x,z)=\frac{1}{\eta_0}(\mathbf{a}_{n_i}\times E_i(x,z))=\left(\frac{\mathbf{a}_z}{20\pi}-\frac{\mathbf{a}_x}{15\pi}\right)e^{-j(6x+8z)},$$
$$\mathbf{H}_i(x,z,t)=\text{Re}[\mathbf{H}_i(x,z)e^{j\omega t}]=\left(\frac{\mathbf{a}_z}{20\pi}-\frac{\mathbf{a}_x}{15\pi}\right)\cos(\num{3e9}t-6x-8z)~\si{\A\per\m}.$$
\item
$$\theta_i=\arccos(\mathbf{a}_n\cdot\mathbf{a}_z)=\arccos0.8\approx0.644~\si{\radian}.$$
\item
$$\mathbf{E}_r(x,z)=-\mathbf{E}_i(x,-z)=-\mathbf{a}_y10e^{-j(6x-8z)},$$
$$\mathbf{a}_{n_r}=\mathbf{a}_x\cdot\frac{k_x}{k}-\mathbf{a}_z\cdot\frac{k_z}{k}$$
$$\mathbf{H}_r(x,z)=\frac{1}{\eta_0}(\mathbf{a}_{n_r}\times E_r(x,z))=-\left(\frac{\mathbf{a}_z}{20\pi}+\frac{\mathbf{a}_x}{15\pi}\right)e^{-j(6x-8z)}.$$
\item
$$\mathbf{E}_1(x,z)=\mathbf{E}_i(x,z)+\mathbf{E}_r(x,z)=-\mathbf{a}_y20je^{-j6x}\sin8z~\si{V\per\m},$$
$$\mathbf{H}_1(x,z)=\mathbf{H}_i(x,z)+\mathbf{H}_r(x,z)=-\frac{\mathbf{a}_z}{10\pi}j\sin8z-\frac{\mathbf{a_x}}{15\pi}2\cos8z.$$
\end{enumerate}


\end{document}
